coq update

code/coq/det.v
@@ -1,26 +1,28 @@
+From Coq Require Import FunctionalExtensionality.
 From mathcomp Require Import all_ssreflect.
 
 From det Require Import program.
 From det Require Import interpreter.
 From det Require Import aux.
 
-Definition functional_goal p :=
+(* Definition functional_prog' p :=
+  forall n r g a, run p n g a = r -> r = None \/ r = Some a. *)
+
+Definition functional_prog p :=
   forall n r g, run p n (not_alt_goal g) [::] = r -> r = None \/ r = Some [::].
 
 Definition functional_pred p f :=
   forall n r, run p n [:: Goal (call f) [::]] [::] = r -> r = None \/ r = Some [::].
 
+Definition functional_goal p g :=
+  forall n r, run p n (not_alt_goal g) [::] = r -> r = None \/ r = Some [::].
+
+Definition functional_goal' p g :=
+  forall n r, run p n (not_alt_goal g) [::] = r -> r = Some [::].
+
+
 Lemma same_int: forall (a:predname), a == a = true.
 Proof. induction a; auto. Qed.
-
-Ltac fold_neck_cut prog f := replace ((fun x' : predname => if f == x' then _ else prog x')) with (neck_cut_pred prog f) by auto.
-Ltac fold_neck_cutH prog f Hyp := replace ((fun x' : predname => if f == x' then _ else prog x')) with (neck_cut_pred prog f) in Hyp by auto.
-
-Ltac fold_neck_cut_all prog := replace (fun x' : predname => [seq cut :: x  | x <- prog x']) with (neck_cut_all prog) by auto.
-Ltac fold_neck_cut_allH prog Hyp := replace (fun x' : predname => [seq cut :: x  | x <- prog x']) with (neck_cut_all prog) in Hyp by auto.
-
-Ltac fold_tail_cut_all prog := replace (fun x' : predname => [seq rcons x cut  | x <- prog x']) with (tail_cut_all prog) by auto.
-Ltac fold_tail_cut_allH prog Hyp := replace (fun x' : predname => [seq rcons x cut  | x <- prog x']) with (tail_cut_all prog) in Hyp by auto.
 
 Lemma not_alt_goal_app:
   forall a b, not_alt_goal a ++ not_alt_goal b = not_alt_goal (a++b).
@@ -30,33 +32,314 @@ Proof.
 Qed.
 
 Lemma functional_neck_cut_all:
-  forall p, functional_goal (neck_cut_all p).
+  forall p, functional_prog (neck_cut_all p).
 Proof.
-  intros prog n.
+  move=> prog n.
   elim: n => /=.
-  - intro; subst; auto.
-  - move=> n IH; destruct r; auto.
-    destruct g as [|g gs]; auto.
-    destruct g.
-    + simpl. intros.
-      eapply IH.
-      apply H.
-    + simpl.
-      unfold neck_cut_all.
-      destruct (prog p) eqn:?; auto.
-      simpl.
-      fold_neck_cut_all prog.
+  - move=> r _ <-; auto.
+  - move=> n IH [sol|]; auto.
+    move=> [|[|p] gs] /=; auto.
+    + apply IH.
+    + simpl; unfold neck_cut_all.
+      destruct (prog p) as [|s] eqn:?; auto.
+      simpl; fold_neck_cut_all prog.
       destruct n; auto.
-      simpl.
-      intros.
+      move => /= H.
       apply pumping1 in H.
-      specialize (IH (Some l) (l0 ++ gs)).
+      specialize (IH (Some sol) (s ++ gs)).
       rewrite <-not_alt_goal_app in IH.
-      apply IH in H.
-      destruct H.
-      by [].
-      inversion H; auto.
+      now apply IH.
 Qed.
+
+Fixpoint has_cut l :=
+  match l with
+  | [::] => False
+  | (cut :: _) => True
+  | _ :: xs => has_cut xs
+  end.
+
+Fixpoint all_has_cut (l: seq (seq pred)) :=
+  match l with
+  | [::] => False
+  | [::x] => has_cut x
+  | [::x&xs] =>
+    has_cut x /\ all_has_cut xs
+  end.
+
+Definition all_have_cut (p: bodiesT) :=
+  forall f, p f <> [::] /\ all_has_cut (p f).
+
+(* Lemma next_alt_help prog p n:
+forall a befs aft l0 r,
+prog p = [::] ->
+  next_alt
+([seq [seq Goal x a  | x <- b] ++
+rcons (not_alt_goal befs) (Goal (call p) [::]) ++ aft
+ | b <- l0] ++ a) (run prog n) = r ->
+  exists n', next_alt a (run prog n') = r.
+Proof.
+Admitted. *)
+
+Lemma cut_does_cut prog n: forall gs befs aft l0 r,
+   run prog n (not_alt_goal (rcons (gs ++ befs) cut ++ aft))
+    [seq [seq Goal x [::]  | x <- b] ++ not_alt_goal (rcons befs cut ++ aft) | b <- l0] = r -> 
+        exists gs', run prog n (not_alt_goal (rcons (gs' ++ befs) cut ++ aft)) [::] = r.
+Proof.
+  induction n.
+  exists [::]; simpl; auto.
+  simpl.
+  destruct gs as [|g gs]; simpl.
+  1:{
+      destruct befs as [|bef befs]; simpl.
+      now exists ([::]).
+      destruct bef as [|p]; [exists [::]; auto|].
+      destruct (prog p) eqn:PP.
+      1:{
+        move => aft [|G GS]; simpl.
+        1:{
+          inversion 1; exists (call p :: [::]); simpl; rewrite PP; auto.
+        }
+        replace  ([seq Goal x [::]  | x <- G] ++ Goal (call p) [::] :: not_alt_goal (rcons befs cut ++ aft)) with
+                (not_alt_goal (rcons (rcons G (call p) ++ befs) cut ++ aft)).
+        2:{
+            rewrite rcons_cat.
+            rewrite <-cats1.
+            do 2 rewrite <-catA.
+            rewrite <-not_alt_goal_app; f_equal.
+          }
+          intros.
+
+          (* apply failing_goal in H.
+          specialize (IHn _ _ _ _ _ H). *)
+          admit.
+      }
+      admit.
+  }
+  admit.
+          
+Admitted.
+
+Lemma func_after_bang prog:
+  forall bef aft,
+    functional_goal prog aft -> 
+      functional_goal prog (rcons bef cut ++ aft).
+Proof.
+  intros.
+  intros ?.
+  revert bef.
+  induction n; auto.
+  simpl.
+  destruct bef as [|bef befs]; simpl.
+  1:{
+      intros.
+      eapply H.
+      apply H0.
+   }
+   destruct bef.
+   1:{
+    apply IHn.
+   }
+   destruct (prog p) eqn:?; auto.
+   intros r.
+   rewrite cats0.
+   rewrite not_alt_goal_app.
+   rewrite catA.
+   rewrite <-rcons_cat.
+   intros.
+   eapply cut_does_cut in H0 as[].
+   epose proof (IHn _ _ H0); auto.
+Qed.
+
+(* Lemma xxxxx gs GS:
+  [seq [seq Goal x [::]  | x <- b] ++ not_alt_goal gs  | b <- [seq rcons x cut  | x <- GS]] =
+  [seq (not_alt_goal (b++gs)) | b <- [seq rcons x cut  | x <- GS]].
+      f_equal.
+      apply functional_extensionality; intros. *)
+
+Lemma map_app {T:Type} {S:Type}:
+  forall (f: T -> S) l1 l2, [seq f x | x <- l1] ++ [seq f x | x <- l2] = [seq f x | x <- l1 ++ l2].
+  Admitted.
+
+(* Lemma pop_goal prog r n:
+  forall g1 a,
+    forall k, run prog k g1 a = Some r
+    -> forall g2, run prog (n+k) (g1 ++ g2) a = Some r.  *)
+
+  (* TODO: if we have bang wherever, then exists one of them
+  producing the same result *)
+
+  (* 
+  
+  run prog n (not_alt_goal (l ++ gs))
+[seq [seq Goal x [::]  | x <- b] ++ not_alt_goal gs
+ | b <- l0] = r
+   *)
+
+
+Lemma all_have_cut'' prog n: forall l l0 ls gs r l1,
+  all_has_cut l1 ->
+    all_has_cut (l::l0)->
+      let T:=[seq [seq Goal x0 [::]  | x0 <- b] ++ not_alt_goal gs  | b <- l1] in
+  run prog n ([seq Goal x T  | x <- l] ++ not_alt_goal (ls ++ gs))
+      ([seq [seq Goal x T  | x <- b] ++ not_alt_goal (ls ++ gs)  | b <- l0] ++ T) =
+r -> exists n', 
+  n' <= n /\
+    run prog n' (not_alt_goal (l ++ gs)) 
+      [seq [seq Goal x [::]  | x <- b] ++ not_alt_goal gs  | b <- l0] = r.
+Proof.
+  simpl; intros.
+  destruct r.
+  2:{ exists 0; auto. }
+Admitted.
+
+Lemma all_have_cut_general prog n:
+all_have_cut prog ->
+    forall gs tl (ll:seq (seq goal)) r, all_has_cut gs ->
+      next_alt [seq [seq Goal x ll | x <- b] ++ tl | b <- gs] (run prog n) = Some r ->
+        exists g n', n' <= n /\ run prog n' ([seq Goal x ll | x <- g] ++ tl) ll = Some r. (*g ∈ gs*)
+Proof.
+
+  (* enough (forall n tl (ll:seq (seq goal)) r, all_has_cut gs ->
+      next_alt [seq not_alt_goal (b++tl) | b <- gs] (run prog n) = Some r ->
+        exists g n', n' <= n /\ run prog n' ([seq Goal x [::] | x <- g]) [::] = Some r (*g ∈ gs*)) by admit.
+  intro. *)
+  intros HProg.
+  induction n; move=> [] // g gs.
+  destruct g.
+  intros; simpl in H; destruct gs; try easy.
+  destruct p.
+  simpl; move=> tl ll r _ H. exists (g), n; constructor; auto.
+
+    
+  destruct (prog p) eqn:PP.
+  simpl; rewrite PP.
+  destruct gs; try by [].
+  move=> tl ll r [C1 C2].
+  simpl.
+  intros.
+  specialize (IHn (l::gs) tl ll r C2).
+
+  simpl in IHn.
+  apply IHn in H as (?&?&?&?).
+  exists x, x0; auto.
+
+  move=> tl ll r H.
+  simpl.
+  rewrite PP.
+  assert (all_has_cut (g::gs)).
+  auto.
+  pose (
+    [seq Goal x [seq [seq Goal x0 ll  | x0 <- b] ++ tl | b <- gs] | x <- l] 
+      ++ [seq Goal x ll  | x <- l] ++ tl) as T.
+  fold T.
+
+  (* rewrite <-map_app. *)
+  (* epose proof (IHn _ ([seq Goal x ll  | x <- l] ++ tl) 
+    ([seq [seq Goal x0 ll  | x0 <- b] ++ tl  | b <- gs]) r H0). *)
+  epose proof (IHn _ _
+    _ r H0).
+  simpl in H1.
+  Unshelve.
+  3:{ apply [seq [seq Goal x0 ll  | x0 <- b] ++ tl  | b <- gs]. }
+  Admitted.
+  
+
+
+
+Lemma all_have_cut' prog n:
+    forall gs tl (ll:seq (seq goal)) r, all_has_cut gs ->
+      next_alt [seq [seq Goal x [::] | x <- b] ++ not_alt_goal tl | b <- gs] (run prog n) = Some r ->
+        exists g n', n' <= n /\ run prog n' ([seq Goal x [::] | x <- g]) [::] = Some r. (*g ∈ gs*)
+Proof.
+
+  (* enough (forall n tl (ll:seq (seq goal)) r, all_has_cut gs ->
+      next_alt [seq not_alt_goal (b++tl) | b <- gs] (run prog n) = Some r ->
+        exists g n', n' <= n /\ run prog n' ([seq Goal x [::] | x <- g]) [::] = Some r (*g ∈ gs*)) by admit.
+  intro. *)
+
+  induction n; move=> [] // g gs.
+  destruct g.
+  intros; simpl in H; destruct gs; try easy.
+  destruct p.
+  simpl; move=> tl _ r _; rewrite map_app; exists (g++tl), n; auto.
+  destruct (prog p) eqn:PP.
+  simpl; rewrite PP.
+  destruct gs; try by [].
+  move=> tl _ r [C1 C2].
+  simpl.
+  intros.
+  specialize (IHn (l::gs) tl [::] r C2).
+
+  simpl in IHn.
+  apply IHn in H as (?&?&?&?).
+  exists x, x0; auto.
+
+  move=> tl _ r H.
+  simpl.
+  rewrite PP.
+  rewrite map_app.
+  simpl.
+  epose proof (IHn _ tl _ r H).
+  simpl in H0.
+
+
+  simpl in H0.
+  (* apply pumping1 in H0. *)
+ 
+
+
+  (* induction eapply IHn; apply H0.
+  destruct (prog p) as [|sol sols] eqn:PP; auto.
+  rewrite cats0.
+  destruct r; auto.
+  intro.
+  unfold not_alt_goal in IHn.
+  specialize (H p) as [? ALL_CUT].
+  rewrite PP in ALL_CUT.
+  pose proof (all_have_cut' _ _ _ _ [::] _ ALL_CUT H0) as [gg[nn [leq HH]]].
+  apply (pumping_leq _ _ _ _ _ _ leq) in HH.
+  now pose proof (IHn _ _ HH).
+Qed. gs as [|g gs]; [by []|]; simpl in *.
+  destruct gs; simpl in *.
+  intros.
+  exists (g ++ tl); simpl.
+  rewrite map_app in H0.
+  exists n; auto.
+  ------
+  destruct H as [CUT_G CUT_GS].
+  specialize (IHgs CUT_GS).
+  intros.
+  repeat rewrite map_app in H.
+  specialize (IHgs (g ++ tl) n ll r). *)
+
+Admitted.
+
+Lemma functional_all_with_cut:
+  forall prog, all_have_cut prog -> functional_prog prog.
+Proof.
+  unfold all_have_cut.
+  intros prog H n.
+  induction n; auto.
+  simpl.
+  destruct g as [|g gs]; simpl; auto.
+  destruct g as [|p].
+
+
+
+Admitted.
+
+  (* intros; eapply IHn; apply H0.
+  destruct (prog p) as [|sol sols] eqn:PP; auto.
+  rewrite cats0.
+  destruct r; auto.
+  intro.
+  unfold not_alt_goal in IHn.
+  specialize (H p) as [? ALL_CUT].
+  rewrite PP in ALL_CUT.
+  pose proof (all_have_cut' _ _ _ _ [::] _ ALL_CUT H0) as [gg[nn [leq HH]]].
+  apply (pumping_leq _ _ _ _ _ _ leq) in HH.
+  now pose proof (IHn _ _ HH).
+Qed. *)
 
 Fixpoint In {A:Type} (a:A) (l:list A) : Prop :=
     match l with
@@ -64,33 +347,7 @@ Fixpoint In {A:Type} (a:A) (l:list A) : Prop :=
       | b :: m => b = a \/ In a m
     end.
 
-(* Lemma InOrNot:
-  forall {T:Type} (e:T) l, In e l \/ not (In e l).
-Proof.
-  induction l; auto.
-  destruct IHl.
-  left.
-  simpl.
-  right.
-  auto.
-  simpl.
-  case (a = e). *)
-
-
-(* 
-  Given some goals G, GS and gs.
-  if (...G, !, gs) each with empty cut-alternatives gives a solution l
-    or one of the alternatives among [(...G1, !, gs), ..., (...GN, !, gs)] with
-      GS = [G1,...,GN] succeeds, then exists at least a succeeding goal G' in [G|GS]
-*)
-
-From Coq Require Import FunctionalExtensionality.
-
-(* Lemma aaa:
-  run (tail_cut_all prog) n (not_alt_goal G') [::] = Some l -> *)
-
-
-Lemma blah prog n l:
+(* Lemma blah prog n l:
   forall G GS gs,
     run (tail_cut_all prog) n (not_alt_goal (rcons G cut ++ gs))
 [seq not_alt_goal (b ++ gs)  | b <- [seq rcons x cut  | x <- GS]] = Some l ->
@@ -129,12 +386,29 @@ Proof.
 
   fold_tail_cut_all prog.
   intros.
-Admitted.
+Admitted. *)
 
+
+(* Lemma all_have_cut_tail_cut_all:
+  forall p, all_have_cut(tail_cut_all p).
+Proof.
+  unfold tail_cut_all.
+  intros ??.
+  destruct (p f); simpl; auto.
+  2:{ split; auto. destruct l0. inversion 1.
+      simpl. }
+  split.
+  intros ?.
+  destruct (p f); simpl in H.
+  destruct (rcons_non_empty _ _ H).
+  simpl.
+  induction f. *)
 
 Lemma functional_tail_cut_all:
-  forall p, functional_goal (tail_cut_all p).
+  forall p, functional_prog (tail_cut_all p).
 Proof.
+  (* intros ??.
+  induction n; auto. *)
   intros prog n r.
   elim: n => /=.
   - move => _ ->; auto.
@@ -164,12 +438,7 @@ Proof.
       rewrite H' in H.
       clear H'.
 
-
-      
-      pose proof (blah prog n l G GS gs H) as [].
-      eapply IH'.
-      apply H0.
-Qed.
+Admitted.
 
 
 
